checkpoint MGet progress

external/Goose/github_com/mit_pdos/gokv/memkv.v
@@ -780,16 +780,10 @@ Definition MemKVClerk__Add: val :=
    FIXME: benchmark *)
 Definition MemKVClerk__MGet: val :=
   rec: "MemKVClerk__MGet" "ck" "keys" :=
-    let: "num_left" := slice.len "keys" in
-    let: "num_left_mu" := lock.new #() in
-    let: "num_left_cond" := lock.newCond "num_left_mu" in
     let: "vals" := NewSlice (slice.T byteT) (slice.len "keys") in
-    ForSlice uint64T "i" "k" "keys"
-      (Fork (SliceSet (slice.T byteT) "vals" "i" (MemKVClerk__Get "ck" "k")));;
-    Skip;;
-    (for: (λ: <>, "num_left" > #0); (λ: <>, Skip) := λ: <>,
-      lock.condWait "num_left_cond";;
-      Continue);;
+    std.Multipar (slice.len "keys") (λ: "i",
+      SliceSet (slice.T byteT) "vals" "i" (MemKVClerk__Get "ck" (SliceGet uint64T "keys" "i"))
+      );;
     "vals".
 
 Definition MakeMemKVClerk: val :=
